\documentclass{article}

\usepackage[letterpaper, top=1in, bottom=1in, left=1in, right=1in]{geometry}
\usepackage{physics, amsmath, enumitem, nicefrac, fancyhdr, microtype, hyperref}

\pagestyle{fancy}

\title{Integral Equations}
\author{Laith Toom}
\date{21/2/2023}

\begin{document}
\maketitle
\newpage

\section{What is an Integral Equation?}
When integrating by parts, there are some instances where 
the integral does not cancel out, or in other words, 
neither $du$ nor $dv$ approach 0. In order to solve such 
an integral, we need to set the integral equal to a variable.
I will be using $I$ to represent our integrals.

\section{Examples}
Let's evaluate some integrals:
\subsection{Integral A}
\[ I = \int e^{2x}\cos(3x) \,dx \tag{A}\label{A} \]
We will use the following substitutions:
\begin{subequations}
    \begin{align*}
        &u = e^{2x} &du = 2e^{2x} \\
        &v = \int \cos(3x) = \frac{1}{3}\sin(3x) &dv = \cos(3x)
    \end{align*}
    \begin{align}
        \int e^{2x}\cos(3x) \,dx &= e^{2x}\frac{1}{3}\sin(3x) - \int 2e^{2x} \frac{1}{3}\sin(3x) \\
                                 &= \frac{1}{3}e^{2x}\sin(3x) - \frac{2}{3}\int e^{2x} \sin(3x)
        \intertext
        {
        Evaluating $\int e^{2x}\sin(3x) \,dx$:
        \begin{align*}
            &u = e^{2x} &du = 2e^{2x} \\
            &v = \int \sin(3x) = \frac{1}{3}\cos(3x) &dv = \sin(3x)
        \end{align*}
        \begin{align*}
            \int e^{2x}\sin(3x) \,dx &= e^{2x}\frac{1}{3}\cos(3x) - \int 2e^{2x}\frac{1}{3}\cos(3x) \,dx \\[1ex]
                                     &= \frac{1}{3}e^{2x}\cos(3x) - \frac{2}{3}\int e^{2x}\cos(3x) \,dx 
        \end{align*}
        Notice that we have $\int e^{2x}\cos(3x) \,dx$, which is the 
        integral we started with, \hyperref[A]{I}. Doing integration by parts again 
        would only take us back to $I$, this we will substitue our 
        integral in this expression with $I$.
        }
        I &= \frac{1}{3}e^{2x}\sin(3x) - \frac{2}{3}\left[ \frac{1}{3}e^{2x}\cos(3x) - \frac{2}{3}I \right] \\
          &= \frac{1}{3}e^{2x}\sin(3x) - \frac{2}{9}e^{2x}\cos(3x) + \frac{4}{9}I \\
        \Rightarrow -\frac{5}{9}I &= \frac{1}{3}e^{2x}\sin(3x) - \frac{2}{9}e^{2x}\cos(3x) \\
        \Rightarrow I &= -\frac{9}{5}\left[\frac{1}{3}e^{2x}\sin(3x) - \frac{2}{9}e^{2x}\cos(3x)\right]
    \end{align}
    Thus:
    \begin{gather}
        I = \int e^{2x}\cos(3x) \,dx \\
        I = -\frac{9}{5}\left[\frac{1}{3}e^{2x}\sin(3x) - \frac{2}{9}e^{2x}\cos(3x)\right] \\
        \boxed{ \int e^{2x}\cos(3x) = -\frac{9}{5}\left[\frac{1}{3}e^{2x}\sin(3x) - \frac{2}{9}e^{2x}\cos(3x)\right] }
    \end{gather}
\end{subequations}

\end{document}